impl/riscv/rsa_ops.i.dfy
@@ -1,29 +1,31 @@
-include "rv_consts.dfy"
-include "bv_ops.dfy"
-include "rv_ops.dfy"
-include "../lib/powers.dfy"
-include "../lib/congruences.dfy"
-include "../libraries/src/Collections/Sequences/LittleEndianNat.dfy"
+include "../../arch/riscv/machine.s.dfy"
+include "../../lib/signed_bv_ops.dfy"
+include "../../std_lib/src/Collections/Sequences/LittleEndianNat.dfy"
 
 module BASE_32_Seq refines LittleEndianNat {
-    import opened rv_ops
     import opened bv_ops
-    import opened rv_consts
     
     function method BASE(): nat { BASE_32 }
 }
 
 module rsa_ops {
-    import opened rv_consts
     import opened bv_ops
-    import opened rv_ops
-    import opened powers
-    import opened congruences
+    import opened rv_machine
 
     import opened DivMod
     import opened Power
     import opened BASE_32_Seq
     import opened Seq
+
+    function to_nat(xs: seq<uint32>): nat
+    {
+        ToNatRight(xs)
+    }
+
+    function seq_subb(xs: seq<uint32>, ys: seq<uint32>): (seq<uint32>, uint1)
+    {
+        SeqSub(xs, ys)
+    }
 
     /* to_nat definions & lemmas */
 
@@ -35,14 +37,14 @@ module rsa_ops {
          assert BASE() == 0x1_00000000;
      }
  
-//     lemma to_nat_lemma_1(xs: seq<uint32>)
-//         requires |xs| == 2
-//         ensures ToNatRight(xs) == xs[0] + xs[1] * BASE_32
-//     {
-//         reveal ToNatRight();
-//         to_nat_lemma_0(xs[..1]);
-//         reveal Pow();
-//     }
+    lemma to_nat_lemma_1(xs: seq<uint32>)
+        requires |xs| == 2
+        ensures ToNatRight(xs) == xs[0] + xs[1] * BASE_32
+    {
+        reveal ToNatRight();
+        to_nat_lemma_0(xs[..1]);
+        reveal Pow();
+    }
 // 
 //     function seq_subb(xs: seq<uint32>, ys: seq<uint32>) : (seq<uint32>, uint1)
 //         requires |xs| == |ys|
